arrays/spec/add.v
@@ -1,0 +1,398 @@
+From Coq Require Import Sorting.Sorted.
+
+From iris.algebra Require Import auth frac_auth gset.
+From iris.heap_lang Require Import proofmode.
+
+From SkipList.lib Require Import lock misc node_rep node_lt key_equiv.
+From SkipList.arrays Require Import code.
+From SkipList.arrays.inv Require Import list_equiv lazy_inv skip_inv.
+From SkipList.arrays.spec Require Import insert.
+
+
+Local Open Scope Z.
+
+Module AddSpec (Params: SKIP_LIST_PARAMS).
+  Import Params.
+  Module Insert := InsertSpec Params.
+  Export Insert.
+
+  Section Proofs.
+    Context `{!heapGS Σ, !gset_list_unionGS Σ, !lockG Σ}.
+
+    Theorem topLevel_spec (lvl h: nat) (key: Z) (top_head curr: node_rep) (S: gset Z) (q: frac)
+      (bot: bot_gname) (top_sub: sub_gname) (bot_subs: list sub_gname) :
+      {{{
+        skip_list_equiv lvl top_head S q bot (top_sub :: bot_subs)
+        ∗
+        (⌜ curr = top_head ⌝ ∨ own (s_auth top_sub) (◯ {[ curr ]}))
+        ∗
+        ⌜ node_key curr < key < INT_MAX ⌝
+        ∗
+        ⌜ h ≤ lvl ⌝
+      }}}
+        topLevel (rep_to_node curr) #key #h #lvl
+      {{{ curr' top_head' top_sub' bot_subs', RET rep_to_node curr';
+        skip_list_equiv h top_head' S q bot (top_sub' :: bot_subs')
+        ∗
+        ( 
+          skip_list_equiv h top_head' (S ∪ {[ key ]}) q bot (top_sub' :: bot_subs')
+          -∗
+          skip_list_equiv lvl top_head (S ∪ {[ key ]}) q bot (top_sub :: bot_subs)
+        )
+        ∗
+        (⌜ curr' = top_head' ⌝ ∨ own (s_auth top_sub') (◯ {[ curr' ]}))
+        ∗
+        ⌜ node_key curr' < key < INT_MAX ⌝
+      }}}.
+    Proof.
+      iIntros (Φ) "(Hlist & Hown_curr & Hcurr_range & Hh) HΦ".
+      iRevert (curr top_head lvl top_sub bot_subs) "Hlist Hown_curr Hcurr_range Hh HΦ".
+      iLöb as "IH".
+      iIntros (curr top_head lvl top_sub bot_subs) "Hlist #Hown_curr %Hcurr_range %Hh HΦ".
+
+      wp_lam. wp_let. wp_let. wp_let.
+
+      rewrite skip_list_equiv_inv.
+      iDestruct "Hlist" as (P obot) "(Hinv & Hlist)".
+      wp_apply (find_sub_spec with "[Hinv]").
+      { by iFrame "# ∗". }
+
+      iIntros (pred succ) "(%Hrange' & #Hown_pred & #Hown_succ & _)".
+      wp_pures.
+      case_bool_decide as Hcase; wp_if.
+      + inversion Hcase as [Heq]. 
+        assert (h = lvl)%nat as <- by lia.
+        iModIntro; iApply "HΦ". 
+        iFrame "# ∗". 
+        iSplit; last (iPureIntro; lia).
+        iIntros "?"; iFrame.
+      + assert (h ≠ lvl) by congruence.
+        destruct bot_subs as [|bot_sub bot_subs].
+        { iDestruct "Hlist" as "(%Hfalse & _)"; lia. }
+        iDestruct "Hlist" as "(#Hlvl & #Hinv & Hmatch)"; unfold is_top_list.
+
+        wp_bind (BinOp _ _ _).
+        iInv (levelN lvl) as (S' Skeys L) "(Hinv_sub & _)" "Hclose".
+        iDestruct "Hinv_sub" as "(>%Hperm & >%Hsort & >%Hequiv & >Hown_auth & >Hown_toks & Hlist)".
+
+        iDestruct "Hown_pred" as "[%Heq | #Hown_pred]".
+        - wp_op.
+          iMod ("Hclose" with "[Hlist Hown_auth Hown_toks]") as "_".
+          { iNext; iExists S', Skeys, L; by iFrame. }
+          iModIntro.
+
+          assert (lvl - 1 = (lvl - 1)%nat) as -> by lia.
+          iApply ("IH" with "[$] [] [%] [%]").
+          { by iLeft. }
+          { lia. }
+          { lia. }
+
+          iNext. 
+          iIntros (curr' top_head' top_sub' bot_subs').
+          iIntros "(Hlist & Himp & Hown_curr' & Hcurr_range')".
+          iApply "HΦ". iFrame "# ∗".
+        - iDestruct (own_valid_2 with "Hown_auth Hown_pred") 
+            as %[Hvalid%gset_included]%auth_both_valid_discrete.
+
+          rewrite (list_equiv_invert_L lvl L top_head pred); last first.
+          { rewrite Hperm -elem_of_list_In elem_of_elements; set_solver. }
+
+          iDestruct "Hlist" as (? ? ? ?) "(_ & Hpt & _ & Hs & _ & _ & HP & Himp)".
+          iDestruct "HP" as "(Hown_frag & Hown_tok)".
+          assert ({[ pred ]} = {[ pred ]} ⋅ {[ pred ]}) as -> by set_solver.
+          iDestruct "Hown_frag" as "(Hown_frag & Hown_frag_dup)".
+
+          wp_op.
+          iPoseProof ("Himp" with "[$]") as "Hlist".
+          iMod ("Hclose" with "[Hlist Hown_auth Hown_toks]") as "_".
+          { iNext; iExists S', Skeys, L; by iFrame. }
+          iModIntro.
+        
+          assert (lvl - 1 = (lvl - 1)%nat) as -> by lia.
+          iApply ("IH" with "[$] [$] [%] [%]").
+          { lia. }
+          { lia. }
+
+          iNext. 
+          iIntros (curr' top_head' top_sub' bot_subs').
+          iIntros "(Hlist & Himp & Hown_curr' & Hcurr_range')".
+          iApply "HΦ". iFrame "# ∗".
+    Qed.
+
+    Theorem addAll_spec (lvl h: nat) (key: Z) (top_head curr: node_rep) (Skeys: gset Z) (q: frac)
+      (bot: bot_gname) (top_sub: sub_gname) (bot_subs: list sub_gname) :
+      INT_MIN < key < INT_MAX →
+      {{{
+        skip_list_equiv lvl top_head Skeys q bot (top_sub :: bot_subs)
+        ∗
+        (⌜ curr = top_head ⌝ ∨ own (s_auth top_sub) (◯ {[ curr ]}))
+        ∗
+        ⌜ node_key curr < key ⌝
+        ∗
+        ⌜ lvl ≤ h ⌝
+      }}}
+        addAll (rep_to_node curr) #key #h #lvl
+      {{{ (v: val) (n: loc) (new: node_rep), RET v;
+        skip_list_equiv lvl top_head (Skeys ∪ {[ key ]}) q bot (top_sub :: bot_subs)
+        ∗
+        ( 
+          ⌜ v = NONEV ⌝ ∨ 
+          ( 
+            ⌜ v = SOMEV #n ⌝ 
+            ∗ 
+            own (s_auth top_sub) (◯ {[ new ]})
+            ∗ 
+            own (s_toks top_sub) (GSet {[ node_key new ]})
+            ∗ 
+            ⌜ node_key new = key ⌝
+            ∗
+            inv (nodeN n) (node_inv n new)
+            ∗ 
+            n ↦{#lfrac lvl} rep_to_node new
+            ∗
+            (node_next new +ₗ lvl +ₗ 1) ↦∗{#1 / 2} replicate (h - lvl) #()
+            ∗
+            ∃ (γ: gname), 
+              is_lock γ (node_lock new) (in_lock (node_next new) (S h))
+              ∗
+              in_lock (node_next new) (S h)
+              ∗
+              locked γ
+          )
+        )
+      }}}.
+    Proof.
+      iIntros (Hkey_range Φ) "(Hlist & Hown_curr & Hrange & Hh) HΦ".
+      iRevert (Φ curr top_head lvl top_sub bot_subs) "Hlist Hown_curr Hrange Hh HΦ".
+      iLöb as "IH".
+      iIntros (Φ curr top_head lvl top_sub bot_subs) "Hlist #Hown_curr %Hrange %Hh HΦ".
+
+      wp_lam. wp_let. wp_let. wp_let.
+      iPoseProof (skip_list_equiv_inv with "Hlist") as (P obot) "(Hinv & Hlist)".
+      wp_apply (find_sub_spec with "[Hinv]").
+      { iFrame "# ∗". iPureIntro; lia. }
+
+      iIntros (pred succ) "(%Hrange' & #Hown_pred & #Hown_succ & _)".
+      wp_pures. 
+
+      destruct bot_subs as [|bot_sub bot_subs].
+      + iDestruct "Hlist" as "(%Hlvl & (Hown_frag & #Hinv))".
+        rewrite Hlvl; wp_pures.
+
+        wp_apply (tryInsert_spec with "[Hown_frag]").
+        { done. }
+        { iFrame "# ∗". iPureIntro; lia. }
+
+        iIntros (v n new) "((Hown_frac & _) & Hopt)".
+        iApply "HΦ". 
+        rewrite loc_add_0.
+        assert (h - 0 = h)%nat as -> by lia.
+
+        assert (1 / 2 / 2 = lfrac 0%nat)%Qp as ->.
+        {
+          rewrite /lfrac.
+          assert (0 + 2 = 2)%nat as -> by lia.
+          rewrite /= Qp_mul_1_r -Qp_div_div //.
+        }
+
+        by iFrame "# ∗".
+      + iDestruct "Hlist" as "(%Hlvl & #Hinv & Hmatch)"; unfold is_top_list.
+        case_bool_decide as Hcase; wp_if.
+        - exfalso; inversion Hcase; lia.
+        - wp_bind (BinOp _ _ _).
+          iInv (levelN lvl) as (S' Skeys' L) "(Hinv_sub & _)" "Hclose".
+          iDestruct "Hinv_sub" as "(>%Hperm & >%Hsort & >%Hequiv & >Hown_auth & >Hown_toks & Hlist)".
+      
+          iDestruct "Hown_pred" as "[%Heq | #Hown_pred]".
+          * wp_op.
+            iMod ("Hclose" with "[Hlist Hown_auth Hown_toks]") as "_".
+            { iNext; iExists S', Skeys', L; by iFrame. }
+            iModIntro. 
+
+            wp_bind (addAll _ _ _ _).
+            assert (lvl - 1 = (lvl - 1)%nat) as -> by lia.
+            iApply ("IH" with "[$] [] [%] [%]").
+            { by iLeft. }
+            { lia. }
+            { lia. }
+
+            iNext. 
+            iIntros (v n new) "(Hlist & Hopt)".
+            iDestruct "Hopt" as "[%Hopt | (%Hopt & Hown_frag & Hown_tok & %Hkey & #Hinvn & Hn & Hnext & Hlock)]".
+            ++ rewrite Hopt; wp_pures.
+               iModIntro; iApply ("HΦ" $! _ n new).
+               iSplitR ""; last by iLeft.
+               by iFrame "# ∗".
+            ++ rewrite Hopt. wp_pures.
+
+               iDestruct "Hn" as "(Hn & Hn')".
+               assert (lfrac (lvl - 1) / 2 = lfrac lvl)%Qp as ->.
+               {
+                 rewrite /lfrac.
+                 assert (lvl - 1 + 2 = S lvl)%nat as -> by lia.
+                 assert (lvl + 2 = S (S lvl))%nat as -> by lia.
+                 rewrite /= Qp_div_div Qp_mul_comm //.
+               }
+
+               rewrite loc_add_assoc.
+               assert ((lvl - 1)%nat + 1 = lvl) as -> by lia.
+               assert (h - (lvl - 1) = S (h - lvl))%nat as -> by lia.
+               rewrite replicate_S array_cons.
+               iDestruct "Hnext" as "(Hnext & Hreplicate)".
+
+               iDestruct "Hlock" as (γ) "(#Hlock & Hin_lock & Hlocked)".
+               iDestruct "Hin_lock" as (vs) "(Hnext' & %Hlength)".
+               pose proof (list_split vs h lvl) as Hsplit.
+               destruct Hsplit as [next Hsplit]; try lia.
+               destruct Hsplit as [vs1 Hsplit]; destruct Hsplit as [vs2 Hsplit].
+               destruct Hsplit as [Hvs Hsplit]; destruct Hsplit as [Hlength1 Hlength2].
+               rewrite Hvs array_app array_cons Hlength1.
+               iDestruct "Hnext'" as "(Hnext'1 & Hnext' & Hnext'2)".
+               iDestruct (mapsto_agree with "Hnext Hnext'") as %<-.
+               iCombine "Hnext Hnext'" as "Hnext".
+
+               wp_apply (insert_spec with "[Hown_frag Hown_tok Hn' Hnext]").
+               { done. }
+               { 
+                 iFrame "# ∗".
+                 iSplit; first by iLeft.
+                 iPureIntro; lia.
+               }
+
+               iIntros (n') "(Hown_frag & Hown_tok & Hnext)".
+               wp_pures.
+               iModIntro; iApply "HΦ". 
+               iFrame "# ∗". iSplit; first done.
+               iRight. iFrame "# ∗".
+               iSplit; first done. iSplit; first done.
+               iExists γ. iFrame "# ∗".
+
+               iCombine "Hnext'1 Hnext Hnext'2" as "Hnext".
+               rewrite -array_cons -Hlength1 -array_app.
+               iExists (vs1 ++ #n' :: vs2); iFrame.
+               iPureIntro; rewrite app_length cons_length; lia.
+          * iDestruct (own_valid_2 with "Hown_auth Hown_pred") 
+              as %[Hvalid%gset_included]%auth_both_valid_discrete.
+
+            rewrite (list_equiv_invert_L lvl L top_head pred); last first.
+            { rewrite Hperm -elem_of_list_In elem_of_elements; set_solver. }
+
+            iDestruct "Hlist" as (γ ? ? ?) "(_ & Hpt & _ & Hs & _ & _ & HP & Himp)"; clear γ.
+            iDestruct "HP" as "(Hown_frag & Hown_tok)".
+            assert ({[ pred ]} = {[ pred ]} ⋅ {[ pred ]}) as -> by set_solver.
+            iDestruct "Hown_frag" as "(Hown_frag & Hown_frag_dup)".
+            assert ({[ pred ]} = {[ pred ]} ⋅ {[ pred ]}) as <- by set_solver.
+
+            wp_op.
+            iPoseProof ("Himp" with "[$]") as "Hlist".
+            iMod ("Hclose" with "[Hlist Hown_auth Hown_toks]") as "_".
+            { iNext; iExists S', Skeys', L; by iFrame. }
+            iModIntro.
+          
+            wp_bind (addAll _ _ _ _).
+            assert (lvl - 1 = (lvl - 1)%nat) as -> by lia.
+            iApply ("IH" with "[$] [$] [%] [%]").
+            { lia. }
+            { lia. }
+
+            iNext. 
+            iIntros (v n new) "(Hlist & Hopt)".
+            iDestruct "Hopt" as "[%Hopt | (%Hopt & Hown_frag & Hown_tok & %Hkey & #Hinvn & Hn & Hnext & Hlock)]".
+            ++ rewrite Hopt. wp_pures.
+               iModIntro; iApply ("HΦ" $! _ n new).
+               iSplitR ""; last by iLeft.
+               by iFrame "# ∗".
+            ++ rewrite Hopt. wp_pures.
+
+               iDestruct "Hn" as "(Hn & Hn')".
+               assert (lfrac (lvl - 1) / 2 = lfrac lvl)%Qp as ->.
+               {
+                 rewrite /lfrac.
+                 assert (lvl - 1 + 2 = S lvl)%nat as -> by lia.
+                 assert (lvl + 2 = S (S lvl))%nat as -> by lia.
+                 rewrite /= Qp_div_div Qp_mul_comm //.
+               }
+
+               rewrite loc_add_assoc.
+               assert ((lvl - 1)%nat + 1 = lvl) as -> by lia.
+               assert (h - (lvl - 1) = S (h - lvl))%nat as -> by lia.
+               rewrite replicate_S array_cons.
+               iDestruct "Hnext" as "(Hnext & Hreplicate)".
+
+               iDestruct "Hlock" as (γ) "(#Hlock & Hin_lock & Hlocked)".
+               iDestruct "Hin_lock" as (vs) "(Hnext' & %Hlength)".
+               pose proof (list_split vs h lvl) as Hsplit.
+               destruct Hsplit as [next Hsplit]; try lia.
+               destruct Hsplit as [vs1 Hsplit]; destruct Hsplit as [vs2 Hsplit].
+               destruct Hsplit as [Hvs Hsplit]; destruct Hsplit as [Hlength1 Hlength2].
+               rewrite Hvs array_app array_cons Hlength1.
+               iDestruct "Hnext'" as "(Hnext'1 & Hnext' & Hnext'2)".
+               iDestruct (mapsto_agree with "Hnext Hnext'") as %<-.
+               iCombine "Hnext Hnext'" as "Hnext".
+
+               wp_apply (insert_spec with "[Hown_frag Hown_tok Hn' Hnext]").
+               { done. }
+               { iFrame "# ∗". iPureIntro; lia. }
+
+               iIntros (n') "(Hown_frag & Hown_tok & Hnext)".
+               wp_pures.
+               iModIntro; iApply "HΦ". 
+               iFrame "# ∗". iSplit; first done.
+               iRight. iFrame "# ∗".
+               iSplit; first done. iSplit; first done.
+               iExists γ. iFrame "# ∗".
+               
+               iCombine "Hnext'1 Hnext Hnext'2" as "Hnext".
+               rewrite -array_cons -Hlength1 -array_app.
+               iExists (vs1 ++ #n' :: vs2); iFrame.
+               iPureIntro; rewrite app_length cons_length; lia.
+    Qed.
+
+    Theorem add_spec (key: Z) (height: nat) (v: val) (S: gset Z) (q: frac)
+      (bot: bot_gname) (subs: list sub_gname)
+      (Hrange: INT_MIN < key < INT_MAX) 
+      (Hheight: height ≤ MAX_HEIGHT) :
+      {{{ is_skip_list v S q bot subs }}}
+        add v #key #height
+      {{{ (b: bool), RET #b; is_skip_list v (S ∪ {[ key ]}) q bot subs }}}.
+    Proof.
+      iIntros (Φ) "H HΦ".
+      iDestruct "H" as (h head) "(%Hv & Hpt & %Hmin & Hlist)".
+
+      wp_lam. wp_let. wp_let.
+      rewrite -Hv. wp_load. wp_let.
+
+      destruct subs as [|sub subs]; first by iExFalso.
+      wp_apply (topLevel_spec  with "[Hlist]").
+      { iFrame. iSplit; first by iLeft. iPureIntro; lia. }
+
+      iIntros (curr top_head top_sub bot_subs).
+      iIntros "(Hlist & Himp & #Hown_curr & %Hcurr_range)".
+      wp_let.
+
+      wp_apply (addAll_spec with "[Hlist]").
+      { done. }
+      { iFrame "# ∗". iPureIntro; lia. }
+
+      iIntros (s n new) "(Hlist & Hopt)".
+      iPoseProof ("Himp" with "Hlist") as "Hlist".
+      wp_let.
+
+      iDestruct "Hopt" as "[%Hnone | (%Hsome & Hown_frag & Hown_tok & %Heq_key & #Hinvn & Hn & _ & Hlock)]".
+      + rewrite Hnone. wp_match.
+        iModIntro. iApply "HΦ".
+        iExists h, head. by iFrame.
+      + rewrite Hsome. wp_match.
+        iDestruct "Hlock" as (γ) "(#Hlock & Hin_lock & Hlocked)".
+
+        wp_load. wp_lam. wp_pures.
+        wp_apply (release_spec with "[Hin_lock Hlocked]"); first done.
+        { iFrame "# ∗". }
+
+        iIntros "_". wp_pures.
+        iModIntro. iApply "HΦ".
+        iExists h, head. by iFrame.
+    Qed.
+
+  End Proofs.
+End AddSpec.
