arrays/spec/insert.v
@@ -1,0 +1,232 @@
+From Coq Require Import Sorting.Sorted.
+
+From iris.algebra Require Import auth frac_auth gset.
+From iris.heap_lang Require Import proofmode.
+
+From SkipList.lib Require Import lock misc node_rep node_lt key_equiv.
+From SkipList.arrays Require Import code.
+From SkipList.arrays.inv Require Import list_equiv lazy_inv skip_inv. 
+From SkipList.arrays.spec Require Import link.
+
+
+Local Open Scope Z.
+
+Module InsertSpec (Params: SKIP_LIST_PARAMS).
+  Import Params.
+  Module Link := LinkSpec Params.
+  Export Link.
+
+  Section Proofs.
+    Context `{!heapGS Σ, !gset_list_unionGS Σ, !lockG Σ} (lvl: nat).
+
+    Theorem tryInsert_spec (key: Z) (head curr: node_rep) (Skeys: gset Z) (q: frac)
+      (sub: sub_gname) (bot: bot_gname) (h: nat) :
+      INT_MIN < key < INT_MAX →
+      {{{
+        is_bot_list 0 head Skeys q sub bot
+        ∗
+        (⌜ curr = head ⌝ ∨ own (s_auth sub) (◯ {[ curr ]}))
+        ∗
+        ⌜ node_key curr < key ⌝
+      }}}
+        tryInsert (rep_to_node curr) #key #h
+      {{{ (v: val) (n: loc) (new: node_rep), RET v;
+        is_bot_list 0 head (Skeys ∪ {[ key ]}) q sub bot
+        ∗
+        ( 
+          ⌜ v = NONEV ⌝ ∨ 
+          ( 
+            ⌜ v = SOMEV #n ⌝ 
+            ∗ 
+            own (s_auth sub) (◯ {[ new ]})
+            ∗ 
+            own (s_toks sub) (GSet {[ node_key new ]})
+            ∗ 
+            ⌜ node_key new = key ⌝
+            ∗
+            inv (nodeN n) (node_inv n new)
+            ∗ 
+            n ↦{#1 / 2 / 2} rep_to_node new
+            ∗
+            (node_next new +ₗ 1) ↦∗{#1 / 2} replicate h #()
+            ∗
+            ∃ (γ: gname), 
+              is_lock γ (node_lock new) (in_lock (node_next new) (S h))
+              ∗
+              in_lock (node_next new) (S h)
+              ∗
+              locked γ
+          )
+        )
+      }}}.
+    Proof.
+      iIntros (Hkey_range Φ) "(Hlazy & #Hown_curr & %Hrange) HΦ".
+      iDestruct "Hlazy" as "(Hown_frag & #Hinv)".
+      wp_lam. wp_let. wp_let.
+
+      wp_apply findLock_spec.
+      { iFrame "#". iPureIntro; lia. }
+      iIntros (pred succ) "(%Hrange' & #Hown_pred & #Hown_succ & Hlock)".
+      iDestruct "Hlock" as (γ' s h') "(%Hlvl & #Hlock & _ & Hpt & #Hinvs & Hin_lock & Hlocked)".
+      rewrite loc_add_0.
+      assert (h' - 1 - 0 = h' - 1)%nat as -> by lia.
+
+      wp_pures. wp_lam. wp_pures.
+      case_bool_decide as Hcase; wp_if.
+      + assert (key = node_key succ) as Heq by congruence.
+        iDestruct "Hown_succ" as "[Hown_succ|%Hsucc]"; last first.
+        { subst; exfalso. rewrite /node_key/tail/= in Hkey_range; lia. }
+
+        wp_lam. wp_bind (Snd _).
+        iInv (levelN 0) as (S Skeys' L) "(Hinv_sub & Hinv_bot)" "Hclose".
+        iDestruct "Hinv_sub" as "(>%Hperm & >%Hsort & >%Hequiv' & >Hown_auth & >Hown_toks & Hlist)".
+        iDestruct "Hinv_bot" as ">Hown_frac"; unfold bot_list_inv.
+
+        iDestruct (own_valid_2 with "Hown_auth Hown_succ") 
+          as %[Hvalid%gset_included]%auth_both_valid_discrete.
+        iDestruct (own_valid_2 with "Hown_frac Hown_frag") 
+          as %Hsub%frac_auth_included_total%gset_included.
+        iMod (own_update_2 with "Hown_frac Hown_frag") as "[Hown_frac Hown_frag]".
+        { apply frac_auth_update, (gset_local_update_union _ _ {[ key ]}). }
+        assert (key ∈ Skeys') as Hin.
+        { rewrite Heq. eapply key_equiv_in; first done. set_solver. }
+        assert (Skeys' ∪ {[ key ]} = Skeys') as -> by set_solver.
+
+        wp_proj.
+        iMod ("Hclose" with "[Hlist Hown_auth Hown_toks Hown_frac]") as "_".
+        { iNext; iExists S, Skeys', L; by iFrame. }
+        iModIntro.
+
+        wp_apply (release_spec with "[Hlock Hpt Hin_lock Hlocked]"); first done.
+        { 
+          iFrame "# ∗". 
+          iDestruct "Hin_lock" as (vs) "(Hnext & %Hlength)".
+          iCombine "Hpt Hnext" as "Hnext"; rewrite -array_cons.
+          iExists (#s :: vs); iFrame.
+          iPureIntro; rewrite cons_length; lia.
+        }
+
+        iIntros "_". wp_pures.
+        iModIntro. iApply "HΦ".
+        iFrame "# ∗". by iLeft.
+      + assert (key ≠ node_key succ) as Hneq by congruence.
+
+        wp_apply (createAndLink_spec with "[Hpt Hown_frag]").
+        { done. }
+        { iFrame "# ∗". iPureIntro; lia. }
+        
+        iIntros (n new) "(Hlazy & Hown_frag & Hown_tok & Hkey & Hpt & Hinvn & Hn & Hnext & Hlock')".
+        wp_let. wp_lam. wp_pures.
+
+        wp_apply (release_spec with "[Hlock Hpt Hin_lock Hlocked]"); first done.
+        { 
+          iFrame "# ∗". 
+          iDestruct "Hin_lock" as (vs) "(Hnext & %Hlength)".
+          iCombine "Hpt Hnext" as "Hnext"; rewrite -array_cons.
+          iExists (#n :: vs); iFrame.
+          iPureIntro; rewrite cons_length; lia.
+        }
+
+        iIntros "_". wp_pures.
+        iModIntro. iApply "HΦ".
+        iFrame. iRight; by iFrame.
+    Qed.
+
+    Theorem insert_spec (key: Z) (head curr new: node_rep) 
+      (top bot: sub_gname) (γ: gname) (n: loc) (h: nat) :
+      INT_MIN < key < INT_MAX →
+      {{{
+        inv (levelN lvl) (lazy_list_inv lvl head top None (from_top_list bot))
+        ∗
+        (⌜ curr = head ⌝ ∨ own (s_auth top) (◯ {[ curr ]}))
+        ∗
+        ⌜ node_key curr < key ⌝
+        ∗ 
+        own (s_auth bot) (◯ {[ new ]})
+        ∗ 
+        own (s_toks bot) (GSet {[ node_key new ]})
+        ∗ 
+        ⌜ node_key new = key ⌝
+        ∗
+        inv (nodeN n) (node_inv n new)
+        ∗ 
+        n ↦{#lfrac lvl} rep_to_node new
+        ∗
+        (node_next new +ₗ lvl) ↦ #()
+        ∗
+        is_lock γ (node_lock new) (in_lock (node_next new) h)
+        ∗
+        ⌜ lvl < h ⌝
+      }}}
+        insert (rep_to_node curr) #lvl #n
+      {{{ s, RET #();
+        own (s_auth top) (◯ {[ new ]})
+        ∗ 
+        own (s_toks top) (GSet {[ node_key new ]})
+        ∗
+        (node_next new +ₗ lvl) ↦{#1 / 2} #s
+      }}}.
+    Proof.
+      iIntros (Hkey_range Φ) "(#Hinv & #Hown_curr & %Hrange & Hown_frag & Hown_tok & %Hkey & #Hinvn & Hn & Hnext & #Hlock & %Hlvl) HΦ".
+      wp_lam. wp_let. wp_let.
+      wp_load. wp_lam. wp_pures.
+
+      wp_apply findLock_spec.
+      { iFrame "#". iPureIntro; lia. }
+      iIntros (pred succ) "(%Hrange' & #Hown_pred & #Hown_succ & Hlock')".
+      iDestruct "Hlock'" as (γ' s h') "(%Hlvl' & #Hlock' & Hin_lock'1 & Hpt & #Hinvs & Hin_lock'2 & Hlocked')".
+
+      wp_let.
+      wp_bind (Fst _).
+      iInv (levelN lvl) as (S Skeys' L) "(Hinv_sub & _)" "Hclose".
+      iDestruct "Hinv_sub" as "(>%Hperm & >%Hsort & >%Hequiv' & >Hown_auth & >Hown_toks & Hlist)".
+      wp_proj.
+
+      iAssert ⌜ key ≠ node_key succ ⌝%I
+        with "[Hown_auth Hown_succ Hown_tok Hlist]" as %Hneq.
+      {
+        iDestruct "Hown_succ" as "[Hown|%Heq]"; last first.
+        { iPureIntro; rewrite Heq /node_key /=; lia. } 
+
+        iDestruct (own_valid_2 with "Hown_auth Hown") 
+          as %[Hvalid%gset_included]%auth_both_valid_discrete.
+
+        assert (In succ L).
+        { rewrite -elem_of_list_In Hperm elem_of_elements. set_solver. }
+
+        rewrite list_equiv_invert_L; last done.
+        iDestruct "Hlist" as (? ? ? ?) "(_ & _ & _ & _ & _ & _ & HP & _)".
+        iDestruct "HP" as "(_ & Hown_tok')".
+
+        iDestruct (own_valid_2 with "Hown_tok Hown_tok'") as 
+          %Hdisj%gset_disj_valid_op.
+        iPureIntro; set_solver.
+      }
+
+      iMod ("Hclose" with "[Hlist Hown_auth Hown_toks]") as "_".
+      { iNext; iExists S, Skeys', L; by iFrame "# ∗". }
+
+      iModIntro; wp_pures.
+
+      wp_apply (link_spec lvl key head pred new succ with "[Hpt Hn Hnext Hown_frag Hown_tok]").
+      { done. }
+      { iFrame "# ∗"; iPureIntro; lia. }
+
+      iIntros "(Hown_frag & Hown_tok & Hpt & Hnext)".
+      wp_pures. wp_lam. wp_pures.
+      wp_apply (release_spec with "[Hin_lock'1 Hpt Hin_lock'2 Hlocked']"); first done.
+      { 
+        iFrame "# ∗". 
+        iDestruct "Hin_lock'1" as (vs1) "(Hnext1 & %Hlength1)".
+        iDestruct "Hin_lock'2" as (vs2) "(Hnext2 & %Hlength2)".
+        iCombine "Hnext1 Hpt Hnext2" as "Hnext".
+        rewrite -array_cons -Hlength1 -array_app.
+        iExists (vs1 ++ #n :: vs2); iFrame.
+        iPureIntro. rewrite app_length cons_length; lia.
+      }
+
+      iIntros "_". iApply "HΦ". iFrame.
+    Qed.
+
+  End Proofs.
+End InsertSpec.
